Use new more primitive heap_ra

src/heap_ra.v
@@ -1,40 +1,318 @@
-From iris.algebra Require Import gmap_view frac.
-From iris.algebra Require Export dfrac.
-From iris.bi.lib Require Import fractional.
-From iris.proofmode Require Import tactics.
-From iris.base_logic.lib Require Export own.
+From stdpp Require Import countable.
+From stdpp Require Import gmap.
+From iris.algebra Require Export cmra.
+From iris.algebra Require Import proofmode_classes updates frac.
+From iris.algebra Require Import agree.
 From iris.prelude Require Import options.
+From iris.base_logic.lib Require Export own.
+From iris.proofmode Require Import tactics.
 
-(*|
-========
-Heap RA
-========
+(* Something like the product of an auth : option (gmap K V) and frag :
+gmapR K V
 
-We define ghost state for reasoning about the simp_lang heap. This is a
-simplification of gen_heap from Iris, which is what HeapLang uses. We don't
-actually build an RA in this library but wrap gmap_view with lemmas about
-ownership in order to give easy-to-read definitions and easy-to-use lemmas.
-
-If you were instantiating Iris you would probably start with gen_heap, but you
-might deviate from it or add to it for custom program logic features that are
-directly tied to the state.
-|*)
-
-
-(** This file provides a generic mechanism for a language-level point-to
-connective [l ↦{dq} v] reflecting the physical heap.  This library is designed to
-be used as a singleton (i.e., with only a single instance existing in any
-proof), with the [gen_heapG] typeclass providing the ghost names of that unique
-instance.  That way, [mapsto] does not need an explicit [gname] parameter.
-This mechanism is plugged into a language and related to the physical heap
-by using [gen_heap_interp σ] in the state interpretation of the weakest
-precondition. See primitive_laws.v for where that happens.
+We don't have any support for agreement because there are no fractions; all
+ownership is exclusive, it's just sharded over keys.
  *)
+
+Section heap_map.
+  Context {K: Type}
+    `{EqDecision0: !EqDecision K}
+    `{Countable0: !Countable K}
+    {V: Type} `{EqDecision V}.
+
+  Record auth_map_val :=
+    { auth: option (gmap K V);
+      frag: gmap K V;
+    }.
+
+  Inductive heap_map :=
+  | Ok (v: auth_map_val)
+  | Invalid.
+
+  Canonical Structure heap_mapO := leibnizO heap_map.
+
+  Global Instance heap_map_inhabited : Inhabited heap_map := populate Invalid.
+  Local Lemma gmap_eq_dec : EqDecision (gmap K V).
+  Proof using All. apply _. Qed.
+  Global Instance auth_map_eq_dec : EqDecision auth_map_val.
+  Proof using All. solve_decision. Qed.
+  Global Instance heap_map_eq_dec : EqDecision heap_map.
+  Proof using All. solve_decision. Qed.
+
+  Global Instance heap_map_Ok_inj : Inj (=) (=) Ok.
+  Proof. by injection 1. Qed.
+
+  (** An element is valid if it's Ok v and the fragment is contained in the
+  auth. *)
+  Local Instance heap_map_valid_instance : Valid heap_map := λ hm,
+    match hm with
+    | Ok {| auth := Some m; frag := m' |} => m' ⊆ m
+    | Ok {| auth := None; frag := m' |} => True
+    | Invalid => False
+    end.
+
+  Instance heap_map_unit : Unit heap_map := Ok {| auth := None; frag := ∅ |}.
+  Local Instance heap_map_pcore_instance : PCore heap_map := λ hm, Some ε.
+
+  Local Instance heap_map_op_instance : Op heap_map := λ hm1 hm2,
+      match hm1, hm2 with
+      | Ok {| auth := Some m1; frag := m1' |},
+        Ok {| auth := Some m2; frag := m2' |} =>
+        Invalid
+      | Ok {| auth := Some m1; frag := m1' |},
+        Ok {| auth := None; frag := m2' |} =>
+          if decide (m1' ##ₘ m2') then
+            Ok {| auth := Some m1; frag := m1' ∪ m2' |}
+          else Invalid
+      | Ok {| auth := None; frag := m1' |},
+        Ok {| auth := mm2; frag := m2' |} =>
+          if decide (m1' ##ₘ m2') then
+            Ok {| auth := mm2; frag := m1' ∪ m2' |}
+          else Invalid
+      | Invalid, _ => Invalid
+      | _, Invalid => Invalid
+      end.
+
+  Lemma heap_map_unit_ok (hm: heap_map) : ε ⋅ hm = hm.
+  Proof.
+    rewrite /ε /heap_map_unit.
+    rewrite /op /heap_map_op_instance.
+    destruct hm as [[[m|] m'] | ]; auto.
+    - rewrite -> decide_True by apply map_disjoint_empty_l.
+      rewrite map_empty_union //.
+    - rewrite -> decide_True by apply map_disjoint_empty_l.
+      rewrite map_empty_union //.
+  Qed.
+
+  Definition Auth (m: gmap K V) : heap_map := Ok {| auth := Some m; frag := ∅ |}.
+  Definition Frag (m: gmap K V) : heap_map := Ok {| auth := None; frag := m |}.
+
+  Lemma heap_map_frag_op (m1 m2: gmap K V) :
+    m1 ##ₘ m2 →
+    Frag m1 ⋅ Frag m2 = Frag (m1 ∪ m2).
+  Proof.
+    intros Hdisj.
+    rewrite /op /heap_map_op_instance /=.
+    rewrite decide_True //.
+  Qed.
+
+  Lemma heap_map_auth_op (m1 m2: gmap K V) :
+    Auth m1 ⋅ Auth m2 = Invalid.
+  Proof.
+    rewrite /op /heap_map_op_instance //=.
+  Qed.
+
+  Local Lemma heap_map_op_auth_frag (m m': gmap K V) :
+    Auth m ⋅ Frag m' = Ok {| auth := Some m; frag := m'; |}.
+  Proof.
+    rewrite /op /heap_map_op_instance /=.
+    rewrite decide_True.
+    - rewrite map_empty_union //.
+    - apply map_disjoint_empty_l.
+  Qed.
+
+  Ltac map_solver :=
+    repeat match goal with
+      | H: context[_ ##ₘ _] |- _ => rewrite map_disjoint_dom in H
+      | |- context[_ ##ₘ _] => rewrite map_disjoint_dom
+      | H: context[dom (_ ∪ _)] |- _ => rewrite dom_union_L in H
+      | |- context[dom (_ ∪ _)] => rewrite dom_union_L
+      | _ => rewrite map_union_assoc
+      end;
+    set_solver.
+
+  Lemma heap_map_op_comm : Comm (=) (op: heap_map → heap_map → heap_map).
+  Proof.
+    intros hm1 hm2.
+    rewrite /op /heap_map_op_instance.
+    destruct hm1 as [[[m1|] m1']|], hm2 as [[[m2|] m2']|];
+      simpl; auto;
+      repeat (destruct (decide _);
+              destruct_and?; subst);
+      try map_solver.
+    all: rewrite map_union_comm //.
+  Qed.
+
+  Definition heap_map_ra_mixin : RAMixin heap_map.
+  Proof.
+    split; try apply _.
+    - intros hm1 hm2 chm1; rewrite leibniz_equiv_iff; intros <-.
+      rewrite /pcore /heap_map_pcore_instance /=.
+      intros [=]; subst.
+      eexists; eauto.
+    - intros hm1 hm2 hm3.
+      rewrite leibniz_equiv_iff.
+      rewrite /op /heap_map_op_instance.
+      destruct hm1 as [[[m1|] m1']|], hm2 as [[[m2|] m2']|], hm3 as [[[m3|] m3']|];
+        simpl; auto;
+        repeat (destruct (decide _);
+                destruct_and?; subst);
+        try map_solver.
+    - intros hm1 hm2.
+      rewrite leibniz_equiv_iff.
+      rewrite /op /heap_map_op_instance.
+      destruct hm1 as [[[m1|] m1']|], hm2 as [[[m2|] m2']|];
+        simpl; auto;
+        repeat (destruct (decide _);
+                destruct_and?; subst);
+        try map_solver.
+      all: rewrite map_union_comm //.
+    - intros hm1 chm1.
+      rewrite /pcore /heap_map_pcore_instance.
+      intros [=]; subst.
+      rewrite heap_map_unit_ok //.
+    - intros hm1 chm1.
+      rewrite /pcore /heap_map_pcore_instance.
+      intros [=]; subst; auto.
+    - intros ??? Hincl.
+      rewrite /pcore /heap_map_pcore_instance => [= <-].
+      eexists; intuition eauto.
+      exists ε; rewrite heap_map_unit_ok //.
+    - intros [[mm1 m1']|] [[mm2 m2']|];
+        rewrite /valid /heap_map_valid_instance /=;
+        rewrite /op /heap_map_op_instance /=;
+        auto.
+      + destruct mm1 as [m1|], mm2 as [m2|]; intuition eauto.
+        revert H; destruct (decide _); intuition eauto.
+        rewrite map_subseteq_spec in H.
+        apply map_subseteq_spec.
+        intros k v Hlookup.
+        apply H.
+        rewrite lookup_union_l //.
+        apply map_disjoint_dom in m.
+        apply elem_of_dom_2 in Hlookup.
+        apply not_elem_of_dom.
+        set_solver.
+      + destruct mm1 as [m1|]; intuition eauto.
+  Qed.
+  Canonical Structure heap_mapR := discreteR heap_map heap_map_ra_mixin.
+
+  Global Instance heap_map_cmra_discrete : CmraDiscrete heap_mapR.
+  Proof. apply discrete_cmra_discrete. Qed.
+
+  Global Instance heap_map_cmra_total : CmraTotal heap_mapR.
+  Proof. intros hm. auto. Qed.
+
+  (* this is the key lemma for creating this RA in the first place *)
+  Lemma heap_map_auth_valid m : ✓ (Auth m).
+  Proof.
+    rewrite /valid /heap_map_valid_instance /Auth.
+    apply map_empty_subseteq.
+  Qed.
+
+  Lemma heap_map_auth_frag_valid m m' : ✓ (Auth m ⋅ Frag m') ↔ m' ⊆ m.
+  Proof.
+    rewrite heap_map_op_auth_frag.
+    rewrite /valid //=.
+  Qed.
+
+  Lemma heap_map_auth_other_valid m hm :
+    ✓ (Auth m ⋅ hm) ↔ ∃ m', hm = Frag m' ∧ m' ⊆ m.
+  Proof.
+    split.
+    - rewrite /valid /heap_map_valid_instance.
+      rewrite /Auth.
+      destruct hm as [[mm' m'']|]; simpl; try solve [ intuition idtac ].
+      destruct mm' as [m'|]; simpl; try solve [ intuition idtac ].
+      rewrite /op /=.
+      rewrite -> decide_True by apply map_disjoint_empty_l.
+      rewrite map_empty_union.
+      intros Hsub.
+      rewrite /Frag. eexists; split; eauto.
+    - intros [m' [-> Hsub]].
+      rewrite heap_map_auth_frag_valid //.
+  Qed.
+
+  Lemma heap_map_frag_frag_valid m m' :
+    ✓ (Frag m ⋅ Frag m') ↔ m ##ₘ m'.
+  Proof.
+    split.
+    - rewrite /Frag /valid /heap_map_valid_instance /=.
+      rewrite /op /=.
+      destruct (decide _); intuition eauto.
+    - intros.
+      rewrite heap_map_frag_op //.
+  Qed.
+
+  Lemma heap_map_auth_frag_other_valid m m' hm :
+    ✓ (Auth m ⋅ Frag m' ⋅ hm) ↔ ∃ m'', hm = Frag m'' ∧ m' ∪ m'' ⊆ m ∧ m' ##ₘ m''.
+  Proof.
+    split.
+    - intros Hval.
+      assert (✓ (Auth m ⋅ hm)).
+      { rewrite -assoc_L (comm _ (Frag m')) assoc_L in Hval.
+        apply cmra_valid_op_l in Hval; auto. }
+      apply heap_map_auth_other_valid in H as [m'' [-> Hsub]].
+      assert (m' ##ₘ m'').
+      { rewrite -assoc_L in Hval; apply cmra_valid_op_r in Hval.
+        apply heap_map_frag_frag_valid in Hval; auto. }
+      rewrite -assoc_L in Hval.
+      rewrite heap_map_frag_op // in Hval.
+      apply heap_map_auth_frag_valid in Hval.
+      eexists; intuition eauto.
+    - intros [m'' (-> & Hsub & Hdisj)].
+      rewrite -assoc_L heap_map_frag_op //.
+      apply heap_map_auth_frag_valid; auto.
+  Qed.
+
+  (* this local update permits allocating a points-to fact for a fresh
+  address *)
+  Lemma heap_map_alloc_update m k v :
+    m !! k = None →
+    Auth m ~~> Auth (<[k := v]> m) ⋅ Frag {[k := v]}.
+  Proof.
+    intros Hnotin.
+    assert (m ##ₘ {[k := v]}).
+    { apply map_disjoint_dom.
+      apply not_elem_of_dom in Hnotin.
+      set_solver. }
+    apply cmra_discrete_update.
+    intros hm'; rewrite heap_map_auth_other_valid.
+    intros [m' [-> Hsub]].
+    assert ({[k := v]} ##ₘ m').
+    { apply map_disjoint_dom in H. apply map_disjoint_dom.
+      apply not_elem_of_dom in Hnotin.
+      apply subseteq_dom in Hsub.
+      set_solver. }
+    rewrite -assoc_L.
+    rewrite heap_map_frag_op //.
+    - apply heap_map_auth_frag_valid.
+      rewrite insert_union_singleton_l.
+      apply map_union_mono_l; auto.
+  Qed.
+
+  Lemma heap_map_modify_update m k v v' :
+    Auth m ⋅ Frag {[k := v]} ~~> Auth (<[k := v']> m) ⋅ Frag {[k := v']}.
+  Proof.
+    apply cmra_discrete_update.
+    intros hm.
+    rewrite ?heap_map_auth_frag_other_valid.
+    intros [m'' (-> & Hsub & Hdisj)].
+    exists m''; intuition eauto.
+    - rewrite insert_union_singleton_l.
+      apply map_union_mono_l.
+      apply map_subseteq_spec => k' v'' Hlookup.
+      rewrite map_subseteq_spec in Hsub.
+      apply Hsub.
+      rewrite lookup_union_r //.
+      apply lookup_singleton_None.
+      apply map_disjoint_dom in Hdisj.
+      apply elem_of_dom_2 in Hlookup.
+      set_solver.
+    - apply map_disjoint_dom.
+      apply map_disjoint_dom in Hdisj.
+      set_solver.
+  Qed.
+
+End heap_map.
+
+Arguments heap_map K {EqDecision0 Countable0} V.
+Arguments heap_mapR K {EqDecision0 Countable0} V.
 
 (** The CMRAs we need, and the global ghost names we are using. *)
 
 Class gen_heapGpreS (L V : Type) (Σ : gFunctors) `{Countable L} := {
-  gen_heapGpreS_inG :> inG Σ (gmap_viewR L (leibnizO V));
+  gen_heapGpreS_inG :> inG Σ (heap_mapR L V);
 }.
 
 Class gen_heapGS (L V : Type) (Σ : gFunctors) `{Countable L} := GenHeapGS {
@@ -45,7 +323,7 @@ Global Arguments GenHeapGS L V Σ {_ _ _} _ : assert.
 Global Arguments gen_heap_name {L V Σ _ _} _ : assert.
 
 Definition gen_heapΣ (L V : Type) `{Countable L} : gFunctors := #[
-  GFunctor (gmap_viewR L (leibnizO V))
+  GFunctor (heap_mapR L V)
 ].
 
 Global Instance subG_gen_heapGpreS {Σ L V} `{Countable L} :
@@ -55,27 +333,25 @@ Proof. solve_inG. Qed.
 Section definitions.
   Context `{Countable L, hG : !gen_heapGS L V Σ}.
 
-(*|
-These two definitions are the key idea behind the state interpretation.
-`gen_heap_interp` is the authoritative element of this RA, which will be the
-state interpretation of `σ`, while `mapsto_def` has fragments that live outside
-the state interpretation and are owned by threads. `l ↦ v` will be notation for
-`mapsto`, with a full 1 fraction.
-|*)
+  (*|
+  These two definitions are the key idea behind the state interpretation.
+  `gen_heap_interp` is the authoritative element of this RA, which will be the
+  state interpretation of `σ`, while `mapsto_def` has fragments that live outside
+  the state interpretation and are owned by threads. `l ↦ v` will be notation for
+  `mapsto`, with a full 1 fraction.
+  |*)
 
-  Definition gen_heap_interp (σ : gmap L V) : iProp Σ :=
-    own (gen_heap_name hG) (gmap_view_auth (DfracOwn 1) (σ : gmap L (leibnizO V))).
+    Definition gen_heap_interp (σ : gmap L V) : iProp Σ :=
+      own (gen_heap_name hG) (Auth (σ : gmap L V)).
 
-  Definition mapsto_def (l : L) (dq : dfrac) (v: V) : iProp Σ :=
-    own (gen_heap_name hG) (gmap_view_frag l dq (v : leibnizO V)).
-  Definition mapsto_aux : seal (@mapsto_def). Proof. by eexists. Qed.
-  Definition mapsto := mapsto_aux.(unseal).
-  Definition mapsto_eq : @mapsto = @mapsto_def := mapsto_aux.(seal_eq).
+    Definition mapsto_def (l : L) (v: V) : iProp Σ :=
+      own (gen_heap_name hG) (Frag {[l := v]}).
+    Definition mapsto_aux : seal (@mapsto_def). Proof. by eexists. Qed.
+    Definition mapsto := mapsto_aux.(unseal).
+    Definition mapsto_eq : @mapsto = @mapsto_def := mapsto_aux.(seal_eq).
 End definitions.
 
-Notation "l ↦{ dq } v" := (mapsto l dq v)
-  (at level 20, format "l  ↦{ dq }  v") : bi_scope.
-Notation "l ↦ v" := (mapsto l (DfracOwn 1) v)
+Notation "l ↦ v" := (mapsto l v)
   (at level 20, format "l  ↦  v") : bi_scope.
 
 Section gen_heap.
@@ -85,21 +361,15 @@ Section gen_heap.
   Implicit Types (σ : gmap L V) (l : L) (v : V).
 
   (** General properties of mapsto *)
-  Global Instance mapsto_timeless l dq v : Timeless (l ↦{dq} v).
+  Global Instance mapsto_timeless l v : Timeless (l ↦ v).
   Proof. rewrite mapsto_eq. apply _. Qed.
 
-  Lemma mapsto_valid_2 l dq1 dq2 v1 v2 : l ↦{dq1} v1 -∗ l ↦{dq2} v2 -∗ ⌜✓ (dq1 ⋅ dq2) ∧ v1 = v2⌝.
+  Lemma mapsto_conflict l v1 v2 : l ↦ v1 -∗ l ↦ v2 -∗ False.
   Proof.
     rewrite mapsto_eq. iIntros "H1 H2".
-    iDestruct (own_valid_2 with "H1 H2") as %[??]%gmap_view_frag_op_valid_L.
-    auto.
-  Qed.
-  (** Almost all the time, this is all you really need. *)
-  Lemma mapsto_agree l dq1 dq2 v1 v2 : l ↦{dq1} v1 -∗ l ↦{dq2} v2 -∗ ⌜v1 = v2⌝.
-  Proof.
-    iIntros "H1 H2".
-    iDestruct (mapsto_valid_2 with "H1 H2") as %[_ ?].
-    done.
+    iDestruct (own_valid_2 with "H1 H2") as %Hdisj%heap_map_frag_frag_valid.
+    apply map_disjoint_dom in Hdisj.
+    set_solver.
   Qed.
 
   (** Update lemmas *)
@@ -110,15 +380,17 @@ Section gen_heap.
     iIntros (Hσl). rewrite /gen_heap_interp mapsto_eq /mapsto_def /=.
     iIntros "Hσ".
     iMod (own_update with "Hσ") as "[Hσ Hl]".
-    { eapply (gmap_view_alloc _ l (DfracOwn 1)); done. }
+    { eapply (heap_map_alloc_update _ l); done. }
     iModIntro. iFrame.
   Qed.
 
-  Lemma gen_heap_valid σ l dq v : gen_heap_interp σ -∗ l ↦{dq} v -∗ ⌜σ !! l = Some v⌝.
+  Lemma gen_heap_valid σ l v : gen_heap_interp σ -∗ l ↦ v -∗ ⌜σ !! l = Some v⌝.
   Proof.
     iIntros "Hσ Hl".
     rewrite /gen_heap_interp mapsto_eq.
-    by iDestruct (own_valid_2 with "Hσ Hl") as %[??]%gmap_view_both_valid_L.
+    iDestruct (own_valid_2 with "Hσ Hl") as %Hsub%heap_map_auth_frag_valid.
+    iPureIntro.
+    apply map_singleton_subseteq_l in Hsub; auto.
   Qed.
 
   Lemma gen_heap_update σ l v1 v2 :
@@ -126,9 +398,9 @@ Section gen_heap.
   Proof.
     iIntros "Hσ Hl".
     rewrite /gen_heap_interp mapsto_eq /mapsto_def.
-    iDestruct (own_valid_2 with "Hσ Hl") as %[_ Hl]%gmap_view_both_valid_L.
+    iDestruct (own_valid_2 with "Hσ Hl") as %Hsub%heap_map_auth_frag_valid.
     iMod (own_update_2 with "Hσ Hl") as "[Hσ Hl]".
-    { eapply gmap_view_update. }
+    { eapply heap_map_modify_update. }
     iModIntro. iFrame.
   Qed.
 End gen_heap.
@@ -136,8 +408,8 @@ End gen_heap.
 Lemma gen_heap_init `{Countable L, !gen_heapGpreS L V Σ} σ :
   ⊢ |==> ∃ _ : gen_heapGS L V Σ, gen_heap_interp σ.
 Proof.
-  iMod (own_alloc (gmap_view_auth (DfracOwn 1) (σ : gmap L (leibnizO V)))) as (γ) "Hσ".
-  { exact: gmap_view_auth_valid.  }
+  iMod (own_alloc (Auth (σ : gmap L V))) as (γ) "Hσ".
+  { exact: heap_map_auth_valid.  }
   iExists (GenHeapGS _ _ _ γ).
   done.
 Qed.
